Began converting minter contract to ConCert build_contract form

examples/fac_master/tzwrap/minter/Fees_Interface.v
@@ -1,11 +1,13 @@
 Require Import Blockchain.
 Require Import ZArith.
+Require Import Serializable.
 
 Section Fees_Interface.
 
 Context {BaseTypes : ChainBase}.
+Set Nonrecursive Elimination Schemes.
 
-Record WithdrawTokensParam : Type :=
+Record WithdrawTokensParam :=
      mkWithdrawTokensParam { fa2_tokens : Address ;
                 tokens : list N}.
 
@@ -19,5 +21,14 @@ Inductive WithdrawalEntrypoint :=
 | Withdraw_all_xtz 
 | Withdraw_token (param : WithdrawTokenParam)
 | Withdraw_xtz (tez : N).
+
+Global Instance WithdrawTokensParam_serializable : Serializable WithdrawTokensParam :=
+    Derive Serializable WithdrawTokensParam_rect<mkWithdrawTokensParam>.
+
+Global Instance WithdrawTokenParam_serializable : Serializable WithdrawTokenParam :=
+    Derive Serializable WithdrawTokenParam_rect<mkWithdrawTokenParam>.
+
+Global Instance WithdrawalEntrypoint_serializable : Serializable WithdrawalEntrypoint :=
+    Derive Serializable WithdrawalEntrypoint_rect<Withdraw_all_tokens, Withdraw_all_xtz, Withdraw_token, Withdraw_xtz>.
 
 End Fees_Interface.
